#########################################################################################
#
#  Bathing Water Profile Feature Ontology
#
#########################################################################################

@base                   <http://location.data.gov.uk/def/ef/BathingWaterProfileFeature/> .
@prefix :               <http://location.data.gov.uk/def/ef/BathingWaterProfileFeature/> .

@prefix def-bwp:        <http://environment.data.gov.uk/def/bathing-water-profile/> .

@prefix rdfs:           <http://www.w3.org/2000/01/rdf-schema#> .
@prefix owl:            <http://www.w3.org/2002/07/owl#> .
@prefix xsd:            <http://www.w3.org/2001/XMLSchema#> .
@prefix rdf:            <http://www.w3.org/1999/02/22-rdf-syntax-ns#> .
@prefix skos:           <http://www.w3.org/2004/02/skos/core#> .
@prefix dcterms:        <http://purl.org/dc/terms/> .
@prefix foaf:           <http://xmlns.com/foaf/0.1/> .
@prefix geo:            <http://www.w3.org/2003/01/geo/wgs84_pos#> .
@prefix def-bw:         <http://environment.data.gov.uk/def/bathing-water/> .
@prefix def-bwsp:       <http://location.data.gov.uk/def/ef/SamplingPoint/> .
@prefix source:         <http://environment.data.gov.uk/sources/def/def-feature.ttl> .

<>
      a       owl:Ontology ;
      dcterms:created       "2012-01-26"^^xsd:date;
      dcterms:modified      "2012-01-26"^^xsd:date;
      dcterms:contributor   [foaf:name "Brian McBride"@en];
      # add your names here

      dcterms:license   <http://www.opendatacommons.org/licenses/pddl/1.0/> ;
      owl:versionInfo "0.1"^^xsd:string .


#############################################################
#
#  Feature classes (except sampling point which is defined elsewhere
#
#############################################################

:Feature
    a                owl:Class ;
    rdfs:label       "Feature"@en ;
    rdfs:comment     """Feature is a class of spatial objects representing features that are relevant to a bathing water profile.  An instance of Feature is a version of an instance of EnduringFeature."""@en ;
    rdfs:isDefinedBy  source:
    .

:EnduringFeature
    a                owl:Class ;
    rdfs:label       "Enduring Feature"@en ;
    rdfs:comment     """EnduringFeature is a class whose instances represent enduring features over time.  Instances of Feature are versions of an instance of EnduringFeature."""@en ;
    .

:DO
    a                owl:Class;
    rdfs:label       "Disused Outfall"@en;
    rdfs:comment     """DO is a class of feature whose instances represent the location of disused outfalls."""@en;
    rdfs:subClassOf geo:Point, :Feature ;
    rdfs:isDefinedBy  source:
    .

:ESO
    a                owl:Class;
    rdfs:label       "Emergency or Storm Overflow"@en;
    rdfs:comment     """ESO is a class of feature whose instances represent the location of emergency or storm overflows."""@en;
    rdfs:subClassOf geo:Point, :Feature ;
    rdfs:isDefinedBy  source:
    .

:RSI
    a                owl:Class;
    rdfs:label       "River or Stream Intersection"@en;
    rdfs:comment     """RSI is a class  of features whose instances represent the location where a river or stream intersects a spatial feature of interest."""@en;
    rdfs:subClassOf     geo:Point, :Feature ;
    rdfs:isDefinedBy  source:
    .

:SWO
    a                 owl:Class;
    rdfs:label        "Surface Water Outfall"@en;
    rdfs:comment      """SWO is a class of feature whose instances represent the location of a surface water outfall."""@en;
    rdfs:subClassOf   geo:Point, :Feature ;
    rdfs:isDefinedBy  source:
    .

:TSO
    a                 owl:Class;
    rdfs:label        "Treated Sewage Works Outfall"@en;
    rdfs:comment      """TTSI is a class of feature whose instances represent the location of a treated sewage works outfall."""@en;
    rdfs:subClassOf   geo:Point, :Feature ;
    rdfs:isDefinedBy  source:
    .

