# Saved by TopBraid on Sun Feb 14 13:13:47 GMT 2010
# baseURI: http://reference.data.gov.uk/def/reference/
# imports: http://rdfs.org/ns/void

@prefix :        <http://reference.data.gov.uk/def/reference/> .
@prefix owl:     <http://www.w3.org/2002/07/owl#> .
@prefix rdf:     <http://www.w3.org/1999/02/22-rdf-syntax-ns#> .
@prefix rdfs:    <http://www.w3.org/2000/01/rdf-schema#> .
@prefix skos:    <http://www.w3.org/2004/02/skos/core#> .
@prefix status:  <http://reference.data.gov.uk/def/status/> .
@prefix void:    <http://rdfs.org/ns/void#> .
@prefix xsd:     <http://www.w3.org/2001/XMLSchema#> .

:     rdf:type owl:Ontology ;
      owl:imports <http://rdfs.org/ns/void> .

:Status
      rdf:type rdfs:Class ;
      rdfs:comment "The status of of a URI set or dataset."@en ;
      rdfs:label "Status"@en ;
      rdfs:subClassOf skos:Concept .

:URIset
      rdf:type rdfs:Class ;
      rdfs:comment "A collection of resources that are all the same kind of thing."@en ;
      rdfs:label "URI Set"@en ;
      rdfs:subClassOf void:Dataset .

:itemType
      rdf:type rdf:Property ;
      rdfs:comment "The common class for all the items in this URI set."@en ;
      rdfs:domain :URIset ;
      rdfs:label "Type of Resources"@en ;
      rdfs:range rdfs:Class .

:status
      rdf:type rdf:Property ;
      rdfs:comment "The status of the URI set or dataset."@en ;
      rdfs:label "Status"@en ;
      rdfs:range :Status .

:uriSet
      rdf:type rdf:Property ;
      rdfs:comment "The URI set that this resource is part of."@en ;
      rdfs:label "URI Set"@en ;
      rdfs:range :URIset .

<http://reference.data.gov.uk/def/status>
      rdf:type skos:ConceptScheme ;
      rdfs:label "Statuses"@en ;
      skos:hasTopConcept status:draft , status:final ;
      skos:prefLabel "Statuses"@en .

status:draft
      rdf:type :Status , skos:Concept ;
      rdfs:label "Draft"@en ;
      skos:definition "Drafts have not been through rigourous review. You are encouraged to use them and give feedback about their suitability, but they may be subject to change without warning."@en ;
      skos:prefLabel "Draft"@en ;
      skos:topConceptOf <http://reference.data.gov.uk/def/status> .

status:final
      rdf:type :Status , skos:Concept ;
      rdfs:label "Final"@en ;
      skos:definition "Final URI sets or datasets have been through review and are not expected to change. You are encouraged to use them."@en ;
      skos:prefLabel "Final"@en ;
      skos:topConceptOf <http://reference.data.gov.uk/def/status> .
