@base					<http://location.data.gov.uk/def/ef/SamplingPoint/> .
@prefix :               <http://location.data.gov.uk/def/ef/SamplingPoint/> .

#@prefix sp-rdf:         <http://location.data.gov.uk/sources/def/ef/SamplingPoint.rdf> .
@prefix sp-ttl:         <http://location.data.gov.uk/sources/def/SamplingPoint.ttl> .


# 2010-12-15 (skw)
# Shifted vocabulary root down to ef/SamplingPoint to allow more modular creation and
# management of vocabulary terms
#

# Prefix for Monitoring Point Locations under INSPIRE environmental monitoring facilities theme.


@prefix	loc-sp:		<http://location.data.gov.uk/def/ef/SamplingPoint/> .

@prefix rdfs:    		<http://www.w3.org/2000/01/rdf-schema#> .
@prefix owl:     		<http://www.w3.org/2002/07/owl#> .
@prefix xsd:     		<http://www.w3.org/2001/XMLSchema#> .
@prefix rdf:     		<http://www.w3.org/1999/02/22-rdf-syntax-ns#> .
@prefix qb:      		<http://purl.org/linked-data/cube#> .
@prefix time:	 		<http://www.w3.org/2006/time#> .
@prefix	interval:       <http://reference.data.gov.uk/def/intervals/> .
@prefix skos:   	    <http://www.w3.org/2004/02/skos/core#> .
@prefix dcterms:        <http://purl.org/dc/terms/> .
@prefix foaf:           <http://xmlns.com/foaf/0.1/> .

@prefix sdmx-attribute: <http://purl.org/linked-data/sdmx/2009/sdmx-attribute#> .

@prefix geo:			<http://www.w3.org/2003/01/geo/wgs84_pos#> .
@prefix geometry:		<http://data.ordnancesurvey.co.uk/ontology/geometry/> .

:
      a       owl:Ontology ;
      rdfs:isDefinedBy      sp-ttl: ;
      dcterms:created		"2010-08-29"^^xsd:date;
    dcterms:modified		"2011-08-23"^^xsd:date;
    owl:imports			geometry: ;
    dcterms:contributor	[foaf:mbox "skw@epimorphics.com"; foaf:name "Stuart Williams"@en];
    # add your names here

    dcterms:license 	<http://www.opendatacommons.org/licenses/pddl/1.0/> ;

      owl:versionInfo "0.1"^^xsd:string .


:SamplingPoint
  a				owl:Class;
  rdfs:label		"SamplingPoint"@en;
  rdfs:comment	"A class of spatial objects or feature types representing the location where samples are taken for environmental monitoring purposes."@en;
  rdfs:isDefinedBy	sp-ttl: ;
  rdfs:subClassOf	geo:Point;
  rdfs:seeAlso		<http://www.legislation.gov.uk/uksi/1991/1597/made>,
              <http://www.legislation.gov.uk/uksi/1991/1597/schedule/1/made>,
              <http://www.legislation.gov.uk/uksi/1991/1597/schedule/2/made>,
              <http://www.legislation.gov.uk/uksi/1991/1597/schedule/3/made>,
              <http://eur-lex.europa.eu/LexUriServ/LexUriServ.do?uri=OJ:L:1976:031:0001:0007:EN:PDF>;
  .

:samplingPoint
  a				owl:ObjectProperty;
  rdfs:label		"samplingPoint"@en;
  rdfs:comment	"""The location of a bathing water quality sampling point.
Sampling at high water

The sampling point represents the location along the high water strandline where the average density of bathers is at its highest. As the tide height changes as does the point but only along the axis of the sampling point / line.

Sampling at other times

At other tidal states, take samples along an imaginary line drawn perpendicular to the shoreline, stretching from the designated high water sampling point to the low water mark. The low water mark finishes at a point where the water depth is approximately 1 metre.
"""@en;
  rdfs:isDefinedBy	sp-ttl: ;
  rdfs:range		:SamplingPoint;
  rdfs:seeAlso	<http://www.legislation.gov.uk/uksi/1991/1597/schedule/2/made>;
  .

:samplePointCode
  a	rdfs:Datatype;
  rdfs:comment		"Datatype for use in typed skos:notations"@en;
  rdfs:label			"samplePointCode"@en;
  rdfs:isDefinedBy	sp-ttl: ;
  .

:samplePointNotation
  a					rdf:Property;
  rdfs:isDefinedBy	sp-ttl: ;
  rdfs:subPropertyOf	skos:notation;
  rdfs:domain			:SamplingPoint;
  rdfs:range			:samplePointCode;
  rdfs:label			"samplePointNotation"@en;
  rdfs:comment		"A skos:notation sub property carrying datatyped notations that code sample point spatial object"@en;
  .



<http://www.legislation.gov.uk/uksi/1991/1597/schedule/1/made>
  rdfs:label	"CRITERIA FOR CLASSIFICATION BW1"@en;
    .

<http://www.legislation.gov.uk/uksi/1991/1597/schedule/2/made>
  rdfs:label	"SAMPLING REQUIREMENTS"@en;
    .

<http://www.legislation.gov.uk/uksi/1991/1597/schedule/3/made>
  rdfs:label	"QUALITY AND ADDITIONAL SAMPLING REQUIREMENTS"@en;
    .

<http://eur-lex.europa.eu/LexUriServ/LexUriServ.do?uri=OJ:L:1976:031:0001:0007:EN:PDF>
  rdfs:label	"EC Bathing Water Directive (76/160/EEC)"@en;
  .

<http://www.legislation.gov.uk/uksi/1991/1597/made>
  rdfs:label "The Bathing Waters (Classification) Regulations 1991"@en
  .