@base					<http://location.data.gov.uk/def/ef/ZoneOfInfluence/> .
@prefix :               <http://location.data.gov.uk/def/ef/ZoneOfInfluence/> .

# @prefix zoi-rdf:        <http://location.data.gov.uk/sources/def/ef/ZoneOfInfluence.rdf> .
@prefix zoi-ttl:        <http://location.data.gov.uk/sources/def/ZoneOfInfluence.ttl> .

# Prefix for Zone of Influence extents under INSPIRE environmental monitoring facilities theme.

@prefix	loc-zoi:		<http://location.data.gov.uk/def/ef/ZoneOfInfluence/> .

@prefix rdfs:    		<http://www.w3.org/2000/01/rdf-schema#> .
@prefix owl:     		<http://www.w3.org/2002/07/owl#> .
@prefix xsd:     		<http://www.w3.org/2001/XMLSchema#> .
@prefix rdf:     		<http://www.w3.org/1999/02/22-rdf-syntax-ns#> .
@prefix qb:      		<http://purl.org/linked-data/cube#> .
@prefix time:	 		<http://www.w3.org/2006/time#> .
@prefix	interval:       <http://reference.data.gov.uk/def/intervals/> .
@prefix skos:   	    <http://www.w3.org/2004/02/skos/core#> .
@prefix dcterms:        <http://purl.org/dc/terms/> .
@prefix foaf:           <http://xmlns.com/foaf/0.1/> .

@prefix sdmx-attribute: <http://purl.org/linked-data/sdmx/2009/sdmx-attribute#> .

@prefix geo:			<http://www.w3.org/2003/01/geo/wgs84_pos#> .
@prefix geometry:		<http://data.ordnancesurvey.co.uk/ontology/geometry/> .

:
      a       owl:Ontology ;
      rdfs:isDefinedBy  zoi-ttl: ;
      dcterms:created		"2011-08-19"^^xsd:date;
    dcterms:modified		"2011-08-23"^^xsd:date;
    owl:imports			geometry: ;
    dcterms:contributor	[foaf:mbox "skw@epimorphics.com"; foaf:name "Stuart Williams"@en];
    # add your names here

    dcterms:license 	<http://www.opendatacommons.org/licenses/pddl/1.0/> ;

      owl:versionInfo "0.1"^^xsd:string .


:ZoneOfInfluence
  a				owl:Class;
  rdfs:label		"ZoneOfInfluence";
  rdfs:comment	"A zone of influence is the approximate topographic area which may have an impact of the water quality at a bathing water due to surface run-off from rivers or streams particularly after heavy rainfall."@en;
  rdfs:isDefinedBy	zoi-ttl: ;
  .

:zoneOfInfluence
  a				owl:ObjectProperty;
  rdfs:label		"zoneOfInfluence"@en;
  rdfs:comment	"""A reusable property of associating some thing, typically a bathing water, with a zone of influence spatial object."""@en;
  rdfs:isDefinedBy	zoi-ttl: ;
  rdfs:range		:ZoneOfInfluence;
  .

:zoiCode
  a	rdfs:Datatype;
  rdfs:comment		"Datatype for use in typed skos:notations"@en;
  rdfs:label			"zoiCode"@en;
  rdfs:isDefinedBy	zoi-ttl: ;
  .

:zoiNotation
  a					rdf:Property;
  rdfs:isDefinedBy	zoi-ttl: ;
  rdfs:subPropertyOf	skos:notation;
  rdfs:domain			:ZoneOfInfluence;
  rdfs:range			:zoiCode;
  rdfs:label			"zoiNotation"@en;
  rdfs:comment		"A skos:notation sub property carrying datatyped notations that code zone of influence spatial-objects"@en;
  .
